adding opens and abbrevs for each source-level toplevel declaration to sigelts and to checked files

ocaml/fstar-lib/generated/FStar_SMTEncoding_Encode.ml
@@ -4272,6 +4272,8 @@ and (encode_sigelt' :
                             (se.FStar_Syntax_Syntax.sigmeta);
                           FStar_Syntax_Syntax.sigattrs =
                             (se.FStar_Syntax_Syntax.sigattrs);
+                          FStar_Syntax_Syntax.sigopens_and_abbrevs =
+                            (se.FStar_Syntax_Syntax.sigopens_and_abbrevs);
                           FStar_Syntax_Syntax.sigopts =
                             (se.FStar_Syntax_Syntax.sigopts)
                         } in
@@ -4456,6 +4458,8 @@ and (encode_sigelt' :
                       (se.FStar_Syntax_Syntax.sigmeta);
                     FStar_Syntax_Syntax.sigattrs =
                       (se.FStar_Syntax_Syntax.sigattrs);
+                    FStar_Syntax_Syntax.sigopens_and_abbrevs =
+                      (se.FStar_Syntax_Syntax.sigopens_and_abbrevs);
                     FStar_Syntax_Syntax.sigopts =
                       (se.FStar_Syntax_Syntax.sigopts)
                   } in
