src/syntax/FStar.Syntax.Util.fst
@@ -1743,7 +1743,9 @@ let action_as_lb eff_lid a pos =
     sigquals = [Visible_default ; Action eff_lid];
     sigmeta = default_sigmeta;
     sigattrs = [];
-    sigopts = None; }
+    sigopts = None;
+    sigopens_and_abbrevs = [];
+    }
 
 (* Some reification utilities *)
 let mk_reify t (lopt:option Ident.lident) =
